

Analysis 2 Übungsblatt 4

Aufgabe 1

$$f(x) = x^3 - 7x^2 + 10x = x(x-5)(x-2) \Rightarrow \text{Die Nullstellen}$$

des $f(x)$ auf x -Achse sind $x_1=0$ $x_2=2$ $x_3=5$

$$\Rightarrow \text{Flächen} = \int_0^2 x^3 - 7x^2 + 10x \, dx + \int_2^5 x^3 - 7x^2 + 10x \, dx$$

$$= \left| \frac{1}{4}x^4 - \frac{7}{3}x^3 + 5x^2 \right|_0^2 + \left| \frac{1}{4}x^4 - \frac{7}{3}x^3 + 5x^2 \right|_2^5$$

$$= \left| \frac{16}{3} - 0 \right| + \left| -\frac{125}{12} - \frac{16}{3} \right|$$

$$= \frac{16}{3} + \frac{189}{12} = \frac{253}{12}$$

Aufgabe 2

$$a) i): \underline{\text{Z:}} \quad x_{n,k} = \frac{k}{n} \quad x_{n,k} - x_{n,k-1} = \frac{k}{n} - \frac{k-1}{n} = \frac{1}{n}$$

$$\Rightarrow \lim_{n \rightarrow \infty} \max_{1 \leq k \leq n} \left| \frac{1}{n} \right| = 0$$

Es sei $\forall \varepsilon > 0, \exists N \in \mathbb{N} = N(\varepsilon), \forall n > N(\varepsilon)$, dass

$$\left| \frac{1}{n} - 0 \right| < \varepsilon \Rightarrow \left| \frac{1}{n} - 0 \right| = \left| \frac{1}{n} \right| < \left| \frac{1}{N(\varepsilon)} \right| = \varepsilon.$$

$$ii): f(x_{n,k}) = f(x_{n,k-1}) = f\left(\frac{k}{n}\right) = \left(\frac{k}{n}\right)^2$$

$$x_{n,k} - x_{n,k-1} = \frac{k}{n} - \frac{k-1}{n} = \frac{1}{n}$$

$$\lim_{n \rightarrow \infty} \sum_{k=1}^n \left(\frac{k}{n}\right)^2 \left(\frac{1}{n}\right) = \lim_{n \rightarrow \infty} \sum_{k=1}^n \frac{k^2}{n^3} = \lim_{n \rightarrow \infty} \frac{1}{n} \sum_{k=1}^n \left(\frac{k}{n}\right)^2$$

$$\sum_{k=1}^n \left(\frac{k}{n}\right)^2 = \int_0^1 x^2 \, dx = \frac{1}{3} x^3 \Big|_0^1 = \frac{1}{3}$$

$$\lim_{n \rightarrow \infty} \frac{1}{n} \cdot \frac{1}{3} = \frac{1}{3} \cdot \lim_{n \rightarrow \infty} \left(\frac{1}{n}\right) = 0 \cdot \frac{1}{3} = 0$$

$$\frac{1}{3} \cdot \lim_{n \rightarrow \infty} \sum_{k=1}^n \frac{1}{n} = \frac{1}{3} \cdot 1 = \frac{1}{3}$$

$$b) i): \tilde{f}: X_{n,k} = (\sqrt[n]{2})^k \quad X_{n,k} - X_{n,k-1} = 2^{\frac{k}{n}} - 2^{\frac{k-1}{n}} = 2^{\frac{k}{n}} (1 - 2^{-\frac{1}{n}})$$

$$\lim_{n \rightarrow \infty} \max_{1 \leq k \leq n} |2^{\frac{k}{n}} (1 - \frac{1}{\sqrt[n]{2}})| = 0$$

Es sei $\forall \varepsilon_1 > 0 \exists N \in \mathbb{N}(\varepsilon_1) \forall n > N(\varepsilon_1)$, dass

$$|(1 - \frac{1}{\sqrt[n]{2}}) - 0| < \varepsilon_1 \Rightarrow |(1 - \frac{1}{\sqrt[n]{2}})| < |(1 - \frac{1}{\sqrt[n]{2}})| = \varepsilon_1$$

$$\Rightarrow \lim_{n \rightarrow \infty} \max_{1 \leq k \leq n} |(1 - \frac{1}{\sqrt[n]{2}})| = 0$$

Es sei $\forall \varepsilon_2 > 0, \exists N \in \mathbb{N}(\varepsilon_2) \forall n > N(\varepsilon_2)$, dass

$$|2^{\frac{k}{n}} - 1| < \varepsilon_2 \Rightarrow |2^{\frac{k}{n}} - 2^0| < |(2^{\frac{k}{n}} - 2^0)| = \varepsilon_2$$

$$\Rightarrow \lim_{n \rightarrow \infty} \max_{1 \leq k \leq n} |2^{\frac{k}{n}}| = 1$$

$$\Rightarrow \lim_{n \rightarrow \infty} \max_{1 \leq k \leq n} |2^{\frac{k}{n}} (1 - \frac{1}{\sqrt[n]{2}})| = 0. \quad \square$$

$$ii): f(x_{n,k}) = \frac{f((\sqrt[n]{2})^k) - 2}{(\sqrt[n]{2})^k} = \frac{f((\sqrt[n]{2})^k)}{(\sqrt[n]{2})^k} = \frac{1}{(\sqrt[n]{2})^{2k}}$$

$$X_{n,k} - X_{n,k-1} = 2^{\frac{k}{n}} (1 - 2^{-\frac{1}{n}})$$

$$\lim_{n \rightarrow \infty} \sum_{k=1}^n f((\sqrt[n]{2})^k) \cdot 2^{\frac{k}{n}} (1 - 2^{-\frac{1}{n}}) \quad \sum_{k=1}^n f(x) = \int_1^2 \frac{1}{x^2} dx = -\frac{1}{x} \Big|_1^2 = \frac{1}{2}$$

$$\lim_{n \rightarrow \infty} \sum_{k=1}^n f(x) (X_{n,k} - X_{n,k-1}) = \lim_{n \rightarrow \infty} \frac{1}{2} \cdot 2^{\frac{k}{n}} (1 - 2^{-\frac{1}{n}})$$

$$= \frac{1}{2} \cdot \lim_{n \rightarrow \infty} 2^{\frac{k}{n}} (1 - 2^{-\frac{1}{n}}) = 0$$

$$= \frac{1}{2} \cdot \lim_{n \rightarrow \infty} \sum_{k=1}^n 2^{\frac{k}{n}} (1 - 2^{-\frac{1}{n}})$$

$$= \frac{1}{2} \sum_{k=1}^n 2^{\frac{k}{n}}$$

$$= \frac{1}{2} \int_0^1 2^x = \frac{1}{2} \cdot \frac{2^x}{\ln 2} \Big|_0^1$$

$$= \frac{1}{2 \cdot \ln 2}$$

$$c) i): \text{Z: } X_{n,k} = 1 + \frac{k}{n} \quad X_{n,k} - X_{n,k-1} = 1 + \frac{k}{n} - (1 + \frac{k-1}{n}) = \frac{1}{n}$$

$$\lim_{n \rightarrow \infty} \max_{1 \leq k \leq n} |X_{n,k} - X_{n,k-1}| = \lim_{n \rightarrow \infty} \max_{1 \leq k \leq n} \left| \frac{1}{n} \right| = 0$$

Es sei $\forall \varepsilon < 0$, $\exists N \in \mathbb{N}(\varepsilon) \quad \forall n > N(\varepsilon)$, dass

$$|(\frac{1}{n}) - 0| < \varepsilon \Rightarrow \left| \frac{1}{n} - 0 \right| = \left| \frac{1}{n} \right| < \left| \frac{1}{N(\varepsilon)} \right| < \varepsilon.$$

$$\Rightarrow \lim_{n \rightarrow \infty} \max_{1 \leq k \leq n} |X_{n,k} - X_{n,k-1}| = 0 \quad \blacksquare$$

$$ii) \quad f(x_{n,k}) = f(\sqrt{X_{n,k-1} X_{n,k}}) = f(\sqrt{(1 + \frac{k-1}{n})(1 + \frac{k}{n})})$$

$$X_{n,k} - X_{n,k-1} = \frac{1}{n}$$

$$\lim_{n \rightarrow \infty} \sum_{k=1}^n f(x) (X_{n,k} - X_{n,k-1}) = \sum_{k=1}^n f(x) = \int_{\frac{1}{2}}^2 \frac{1}{x^2} dx = \left[-\frac{1}{x} \right]_{\frac{1}{2}}^2 = \frac{2-1}{2}$$

$$= \frac{2-1}{2} \lim_{n \rightarrow \infty} \sum_{k=1}^n \left(\frac{1}{n} \right) = \frac{2-1}{2} \cdot 1 = \frac{2-1}{2} = \frac{2-1}{2}$$